src/Executable_Defs_Prop.v
@@ -1,4 +1,4 @@
-Require Import Term_Defs_Core Manifest_Admits Manifest.
+Require Import Term_Defs_Core Manifest_Admits Manifest Params_Admits.
 
 Require Import List.
 Import ListNotations.
@@ -15,6 +15,9 @@ Definition canRunAsp_Manifest(* (k:Plc) *) (m:Manifest)(params:ASP_PARAMS):Prop 
     can_measure_target_prop policyM(*ac_policyM*) targplc targid 
   end.
 
+Definition canRun_aspid (m:Manifest) (i:ASP_ID):Prop :=
+  In i m.(asps).
+
 Definition knowsOf_Manifest(*(k:Plc)*)(e:Manifest)(p:Plc):Prop :=
   In p e.(uuidPlcs).
 
@@ -25,6 +28,8 @@ Fixpoint executable(t:Term)(*(k:Plc)*)(e:Manifest):Prop :=
   match t with
   | asp (ASPC _ _ params)  => canRunAsp_Manifest e params
   | asp (ENC p) => knowsPub_Manifest e p
+  | asp SIG => canRun_aspid e (sig_aspid)
+  | asp HSH => canRun_aspid e (hsh_aspid)
   | asp _ => True
   | att p t => knowsOf_Manifest e p (* -> executable t k e *)
   | lseq t1 t2 => executable t1 e /\ executable t2 e
