src/Executable_Facts.v
@@ -1,5 +1,6 @@
 Require Import Term_Defs_Core Manifest Manifest_Generator (* Manifest_Generator_Facts *) Executable_Defs_Prop Manifest_Admits Eqb_Evidence.
 
+Require Import Params_Admits.
 Require Import List.
 Import ListNotations.
 
@@ -25,17 +26,17 @@ Print Manifest.
 Print Environment.
 *)
 
-Definition canRunAsp_Env (k:Plc) (em:EnvironmentM) (a: ASP_ID) : Prop := 
+Definition canRunAsp_Env (k:Plc) (em:EnvironmentM) (ps: ASP_PARAMS) : Prop := 
   match (Maps.map_get em k) with 
   | None => False 
-  | Some m => In a m.(asps)
+  | Some m => canRunAsp_Manifest m ps
   end. 
   
-  
-Print EnvironmentM.
-(*  Maps.MapC Plc Manifest *)
-
-Print knowsOf_Manifest.
+Definition canRun_aspid_Env (k:Plc) (em:EnvironmentM) (i:ASP_ID) : Prop :=
+  match (Maps.map_get em k) with 
+  | None => False 
+  | Some m => canRun_aspid m i
+  end. 
 
 Definition knowsOf_Env (k:Plc)(em:EnvironmentM)(p:Plc):Prop :=
   match (Maps.map_get em k) with 
@@ -43,10 +44,19 @@ Definition knowsOf_Env (k:Plc)(em:EnvironmentM)(p:Plc):Prop :=
   | Some m => In p m.(uuidPlcs)
   end.
 
+Definition knowsPub_Env (k:Plc)(em:EnvironmentM)(p:Plc):Prop :=
+    match (Maps.map_get em k) with 
+    | None => False
+    | Some m => In p m.(pubKeyPlcs)
+    end.
+
 (* Statically, we have a global view so we can use the environement to reason about the system *)
 Fixpoint executable_static (t:Term) (k:Plc) (em:EnvironmentM) : Prop := 
   match t with
-    | asp (ASPC _ _ (asp_paramsC asp_id _ _ _))  => canRunAsp_Env k em asp_id
+    | asp (ASPC _ _ ps)  => canRunAsp_Env k em ps
+    | asp SIG => canRun_aspid_Env k em (sig_aspid)
+    | asp HSH => canRun_aspid_Env k em (hsh_aspid)
+    | asp (ENC p) => knowsPub_Env k em p
     | asp _ => True
     | att p t1 => knowsOf_Env k em p /\ executable_static t1 p em
     | lseq t1 t2 => executable_static t1 k em /\ executable_static t2 k em
@@ -58,7 +68,12 @@ Fixpoint executable_static (t:Term) (k:Plc) (em:EnvironmentM) : Prop :=
    At runtime, we cannot know if an att term can be executed on a remote place. *)
 Fixpoint executable_dynamic (t:Term) (k:Plc) (em:EnvironmentM) : Prop := 
   match t with
-    | asp (ASPC _ _ (asp_paramsC asp_id _ _ _))  => canRunAsp_Env k em asp_id
+    (* | asp (ASPC _ _ (asp_paramsC asp_id _ _ _))  => canRunAsp_Env k em asp_id
+    | asp _ => True *)
+    | asp (ASPC _ _ ps)  => canRunAsp_Env k em ps
+    | asp SIG => canRun_aspid_Env k em (sig_aspid)
+    | asp HSH => canRun_aspid_Env k em (hsh_aspid)
+    | asp (ENC p) => knowsPub_Env k em p
     | asp _ => True
     | att p t => knowsOf_Env k em p
     | lseq t1 t2 => executable_dynamic t1 k em /\ executable_dynamic t2 k em
