src/Executable_Facts_Dist.v
@@ -1,6 +1,6 @@
 Require Import Term_Defs_Core Manifest Manifest_Generator Manifest_Generator_Facts Executable_Defs_Prop Manifest_Admits Eqb_Evidence.
 
-Require Import Executable_Facts.
+Require Import Executable_Facts Params_Admits.
 
 Require Import StructTactics Auto.
 
@@ -38,11 +38,20 @@ Print Manifest.
 Print Environment.
 *)
 
+(*
 Definition canRunAsp_Env (k:Plc) (em:EnvironmentM) (a: ASP_ID) : Prop := 
   match (Maps.map_get em k) with 
   | None => False 
   | Some m => In a m.(asps)
   end. 
+*)
+
+
+Definition canRunAsp_Env (k:Plc) (em:EnvironmentM) (ps: ASP_PARAMS) : Prop := 
+    match (Maps.map_get em k) with 
+    | None => False 
+    | Some m => canRunAsp_Manifest m ps
+end. 
 
 Definition knowsOf_Env (k:Plc)(em:EnvironmentM)(p:Plc):Prop :=
   match (Maps.map_get em k) with 
@@ -50,6 +59,8 @@ Definition knowsOf_Env (k:Plc)(em:EnvironmentM)(p:Plc):Prop :=
   | Some m => In p m.(uuidPlcs)
   end.
 
+
+  (*
 (* Statically, we have a global view so we can use the environement to reason about the system *)
 Fixpoint executable_static (t:Term) (k:Plc) (em:EnvironmentM) : Prop := 
   match t with
@@ -61,9 +72,40 @@ Fixpoint executable_static (t:Term) (k:Plc) (em:EnvironmentM) : Prop :=
     | bseq _ t1 t2 => executable_static t1 k em /\ executable_static t2 k em
     | bpar _ t1 t2 => executable_static t1 k em /\ executable_static t2 k em
   end.
+  *)
+
+  Fixpoint executable_static (t:Term) (k:Plc) (em:EnvironmentM) : Prop := 
+    match t with
+      | asp (ASPC _ _ ps)  => canRunAsp_Env k em ps
+      | asp SIG => canRun_aspid_Env k em (sig_aspid)
+      | asp HSH => canRun_aspid_Env k em (hsh_aspid)
+      | asp (ENC p) => knowsPub_Env k em p
+      | asp _ => exists m, Maps.map_get em k = Some m
+      | att p t1 => knowsOf_Env k em p /\ executable_static t1 p em
+      | lseq t1 t2 => executable_static t1 k em /\ executable_static t2 k em
+      | bseq _ t1 t2 => executable_static t1 k em /\ executable_static t2 k em
+      | bpar _ t1 t2 => executable_static t1 k em /\ executable_static t2 k em
+    end.
+
 
 (* A dynamic version of executabiilty. 
    At runtime, we cannot know if an att term can be executed on a remote place. *)
+
+   Fixpoint executable_dynamic (t:Term) (k:Plc) (em:EnvironmentM) : Prop := 
+    match t with
+      (* | asp (ASPC _ _ (asp_paramsC asp_id _ _ _))  => canRunAsp_Env k em asp_id
+      | asp _ => True *)
+      | asp (ASPC _ _ ps)  => canRunAsp_Env k em ps
+      | asp SIG => canRun_aspid_Env k em (sig_aspid)
+      | asp HSH => canRun_aspid_Env k em (hsh_aspid)
+      | asp (ENC p) => knowsPub_Env k em p
+      | asp _ => True
+      | att p t => knowsOf_Env k em p
+      | lseq t1 t2 => executable_dynamic t1 k em /\ executable_dynamic t2 k em
+      | bseq _ t1 t2 => executable_dynamic t1 k em /\ executable_dynamic t2 k em
+      | bpar _ t1 t2 => executable_dynamic t1 k em /\ executable_dynamic t2 k em
+    end.
+(*
 Fixpoint executable_dynamic (t:Term) (k:Plc) (em:EnvironmentM) : Prop := 
   match t with
     | asp (ASPC _ _ (asp_paramsC asp_id _ _ _))  => canRunAsp_Env k em asp_id
@@ -73,6 +115,7 @@ Fixpoint executable_dynamic (t:Term) (k:Plc) (em:EnvironmentM) : Prop :=
     | bseq _ t1 t2 => executable_dynamic t1 k em /\ executable_dynamic t2 k em
     | bpar _ t1 t2 => executable_dynamic t1 k em /\ executable_dynamic t2 k em
   end.
+  *)
 
 (*
 Definition envs_eq_at (e:Environment) (em:EnvironmentM) (ps:list Plc) : Prop := 
@@ -109,7 +152,7 @@ Theorem static_executability_implies_dynamic :
       executable_dynamic t p em.
 Proof.
   intros t. induction t; try ( intros; inversion H; specialize IHt1 with p em; specialize IHt2 with p em; simpl; split; auto).
-  + intros. destruct a; try (apply I). auto.
+  + intros. destruct a; try (apply I); auto.
   + intros. specialize IHt with p0 em. simpl in *. inversion H. apply H0.
 Qed. 
 
@@ -922,40 +965,47 @@ Proof.
       exists m. 
       split; try eauto.
       door; ff.
+      (*
       rewrite <- H0.
       cbn.
       break_let; ff. subst.
       split; try eassumption.
       cbv.
-      trivial.
-    + unfold distributed_executability; intros.
-      invc H.
+      trivial. *)
+
+      + unfold distributed_executability; intros.
+      subst.
       ff.
       destruct_conjs.
       door; ff; subst.
-      exists x.
-      split; try eauto.
       door; ff; subst.
-      unfold executable.
-      trivial.
-    + unfold distributed_executability; intros.
-      invc H.
+      unfold canRun_aspid_Env in H.
+      ff.
+      exists m. 
+      split; try eauto.
+
+      + unfold distributed_executability; intros.
+      subst.
       ff.
       destruct_conjs.
       door; ff; subst.
-      exists x.
-      split; try eauto.
       door; ff; subst.
-      unfold executable.
-      trivial.
-    + unfold distributed_executability; intros.
-      invc H.
+      unfold canRun_aspid_Env in H.
+      ff.
+      exists m. 
+      split; try eauto.
+
+      + unfold distributed_executability; intros.
+      subst.
       ff.
       destruct_conjs.
       door; ff; subst.
-      exists x.
-      split; try eauto.
       door; ff; subst.
+      unfold knowsPub_Env in H.
+      ff.
+      exists m. 
+      split; try eauto.
+      
   - (* at case *)
     simpl in *.
     invc H.
